\paragraph{Example}
$$X \sim U([0,1]) \quad Y|X \sim U([0,x])$$
\subparagraph{Solution}
$f_X(x) = 1 \quad 0\leq x\leq 1$ and $f_{Y|X}f_X(x)=\frac{1}{x} \quad 0\leq y \leq x$.
Thus
$$f(x,y) = f_X(x) f_{Y|X} (y|x) = \frac{1}{x} \quad 0\leq y \leq x \leq 1$$
And
$$f_Y(y) = \int_{-\infty}^{\infty} f(x,y) dx = \int_y^1 \frac{1}{x} = -\log y \quad 0\leq y \leq 1 $$
\paragraph{Exercise}
Find $\mathbb{E}Y$
\subparagraph{Solution}
$$\mathbb{E}Y = \int_0^1 y (-\log y)dy  = -\int_0^1 y\log y dy = \frac{1}{4}$$

\paragraph{Linearity of expectation}
Define $\Psi(X,Y) = X+Y$.

Then
\begin{align*}
\mathbb{E} (X+Y) = \mathbb{E} \Psi (X,Y)= \int_{-\infty}^{\infty}\int_{-\infty}^{\infty} \Psi(x,y)f(x,y) dx dy = \int_{-\infty}^{\infty} dx x\int_{-\infty}^{\infty}  dy f(x,y) + \int_{-\infty}^{\infty}dy y\int_{-\infty}^{\infty} dx f(x,y)   =\\= \int_{-\infty}^{\infty} x f_X(x)dx + \int_{-\infty}^{\infty} y f_Y(y) dy = \mathbb{E}X +\mathbb{E}Y
\end{align*}
\paragraph{Sum of independent variables}
Suppose $X,Y$ independent. 
$$f(x,y) = f_X(x) f_Y(y)$$
$$p(x,y) = p_X(x) p_Y(y)$$
We denote $Z=X+Y$ and want to find $f_Z(z) = f_{X+Y}(z) = ?$

\subparagraph{Discrete}
$$p_Z(z)=p_{X+Y}(z) = P(X+Y=z) = \sum_x P(X=x, Y=z-x) \stackrel{ind}{=} \sum_x P(X=x) P(Y=z-x) = \sum_x p_x(x) p_y(z-x)$$
\subparagraph{Continuous}
 Denote $A_z = \left\{ (x,y) : x+y \leq z \right\}$. Then
\begin{align*}
F_{X+Y} (z) = P(X+Y\leq z) = P((X,Y) \in A_z) = \iint\limits_{A_z} f(x,y) dxdy = \int_{-\infty}^{\infty} dx \int_{-\infty}^{z-x} dy f(x,y) \stackrel{ind}{=}\\= \int_{-\infty}^{\infty} dx \int_{-\infty}^{z-x} dy f_X(x)f_Y(y) = \int_{-\infty}^{\infty} dx f_X(x) \int_{-\infty}^{z-x} dy f_Y(y) 
\end{align*}
$$$$
Then
$$f_{X+Y}(z) = \frac{d}{dz} \int_{-\infty}^{\infty} dx f_X(x) \int_{-\infty}^{z-x} dy f_Y(y) = \int_{-\infty}^\infty f_X(x) f_Y(z-x) dx = \left( f_X * f_Y \right)(z)$$